submaps, note doesn't build

deps/poulet4/lib/Maps.v
@@ -78,6 +78,21 @@ Module FuncAsMap.
                        k <> k' -> get k (set k' v m) = get k m.
     Proof. intros. unfold set, get. specialize (H _ _ H0). now rewrite H. Qed.
 
+    (** [m1 ⊆ m2]. *)
+    Definition submap (m1 m2 : t) : Prop :=
+      forall k v, m1 k = Some v -> m2 k = Some v.
+
+    Lemma submap_eq : forall m1 m2 k,
+        submap m1 m2 -> submap m2 m1 -> m1 k = m2 k.
+    Proof.
+      unfold submap.
+      intros m1 m2 k Hsub1 Hsub2.
+      destruct (m1 k) as [v |] eqn:Hm1k.
+      - symmetry; auto.
+      - destruct (m2 k) as [v |] eqn:Hm2k; try reflexivity.
+        apply Hsub2 in Hm2k.
+        rewrite Hm1k in Hm2k; discriminate.
+    Qed.
   End FuncAsMap.
 
   Section FuncMapMap.
